SampCert/DifferentialPrivacy/Queries/UnboundedMax/Basic.lean
@@ -1,10 +1,13 @@
 /-
 Copyright (c) 2024 Amazon.com, Inc. or its affiliates. All Rights Reserved.
 Released under Apache 2.0 license as described in the file LICENSE.
-Authors: Jean-Baptiste Tristan
+Authors: Markus de Medeiros
 -/
 
 -- import SampCert.DifferentialPrivacy.Queries.UnboundedMax.Code
--- import SampCert.DifferentialPrivacy.Queries.UnboundedMax.Properties
+
+import SampCert.DifferentialPrivacy.Queries.UnboundedMax.Properties
+import SampCert.DifferentialPrivacy.Queries.UnboundedMax.Privacy
+
 -- import SampCert.DifferentialPrivacy.Queries.UnboundedMax.Pure
 -- import SampCert.DifferentialPrivacy.Queries.UnboundedMax.ZeroConcentrated
